Make typing lemmas about continuations and functions easier to apply.
By letting them only speak about lits in their conclusions, and use [length] as the length parameter of vec. Also simplified substitutions of vectors.

theories/lang/lang.v
@@ -163,15 +163,14 @@ Fixpoint subst_l (xl : list binder) (esl : list expr) (e : expr) : option expr :
   | _, _ => None
   end.
 
-Definition subst_vec {n} (xl : vec binder n) (el : vec expr n) : expr → expr :=
-  Vector.rect2 (λ _ _ _, expr → expr) id
-               (λ n _ _ rec x e, rec ∘ subst' x e) xl el.
-
-Lemma subst_vec_eq {n} (xl : vec binder n) (el : vec expr n) e :
-  Some $ subst_vec xl el e = subst_l xl el e.
+Definition subst_v (xl : list binder) (esl : vec expr (length xl))
+                   (e : expr) : expr :=
+  from_option id (Var "" (* Dummy *)) (subst_l xl esl e).
+Lemma subst_v_eq (xl : list binder) (esl : vec expr (length xl)) e :
+  Some $ subst_v xl esl e = subst_l xl esl e.
 Proof.
-  revert n xl el e. eapply (vec_rect2 (λ n xl el, ∀ e, Some $ subst_vec xl el e = subst_l xl el e)); first done.
-  move=>n xl el IH x es e. simpl. apply IH.
+  unfold subst_v. destruct subst_l eqn:EQ; first done. exfalso. revert esl e EQ.
+  induction xl=>/= esl; inv_vec esl; first done. simpl. eauto.
 Qed.
 
 (** The stepping relation *)
@@ -501,14 +500,6 @@ Qed.
 Lemma stuck_not_head_step σ e' σ' ef :
   ¬head_step stuck_term σ e' σ' ef.
 Proof. inversion 1. Qed.
-
-Lemma Forall_of_val_is_val l :
-  Forall (λ ei : expr, is_Some (to_val ei)) (of_val <$> l).
-Proof.
-  induction l; constructor.
-  - rewrite to_of_val. eauto.
-  - apply IHl.
-Qed.
 
 (** Equality and other typeclass stuff *)
 Instance base_lit_dec_eq : EqDecision base_lit.
