theories/typing/cont.v
@@ -8,34 +8,34 @@ Section typing.
   Context `{typeG Σ}.
 
   (** Jumping to and defining a continuation. *)
-  Lemma type_jump {n} E L k T' T (args : vec val n) :
-    tctx_incl E L T (T' args) →
-    typed_body E L [CCtx_iscont k L n T'] T (k (of_val <$> (args : list _))).
+  Lemma type_jump E L C T k args T' :
+    CCtx_iscont k L _ T' ∈ C →
+    tctx_incl E L T (T' (list_to_vec args)) →
+    typed_body E L C T (k (of_val <$> args)).
   Proof.
-    iIntros (Hincl tid qE) "#HEAP #LFT Htl HE HL HC HT".
+    iIntros (HC Hincl tid qE) "#HEAP #LFT Htl HE HL HC HT".
     iMod (Hincl with "LFT HE HL HT") as "(HE & HL & HT)".
-    iSpecialize ("HC" with "HE * []"); first by (iPureIntro; apply elem_of_list_singleton).
-    simpl. iApply ("HC" with "* Htl HL HT").
+    iSpecialize ("HC" with "HE * []"); first done.
+    rewrite -{3}(vec_to_list_of_list args). iApply ("HC" with "* Htl HL HT").
   Qed.
 
-  Lemma type_cont {n} E L1 L2 C T T' kb (argsb : vec binder n) e1 econt e2 :
-    e1 = Rec kb argsb econt → Closed (kb :b: argsb +b+ []) econt → Closed (kb :b: []) e2 →
-    (∀ k args, typed_body E L1 (CCtx_iscont k L1 n T' :: C) (T' args)
-                          (subst' kb k $ subst_vec argsb (Vector.map of_val $ args) econt)) →
-    (∀ k, typed_body E (L1 ++ L2) (CCtx_iscont k L1 n T' :: C) T (subst' kb k e2)) →
-    typed_body E (L1 ++ L2) C T (let: kb := e1 in e2).
+  Lemma type_cont E L1 L2 C T argsb econt e2 T' kb :
+    Closed (kb :b: argsb +b+ []) econt → Closed (kb :b: []) e2 →
+    (∀ k args, typed_body E L1 (CCtx_iscont k L1 _ T' :: C) (T' args)
+                          (subst' kb k $ subst_v argsb (vmap of_val args) econt)) →
+    (∀ k, typed_body E (L1 ++ L2) (CCtx_iscont k L1 _ T' :: C) T (subst' kb k e2)) →
+    typed_body E (L1 ++ L2) C T (let: kb := Rec kb argsb econt in e2).
   Proof.
-    iIntros (-> Hc1 Hc2 Hecont He2 tid qE) "#HEAP #LFT Htl HE HL HC HT". iApply wp_let'.
+    iIntros (Hc1 Hc2 Hecont He2 tid qE) "#HEAP #LFT Htl HE HL HC HT". iApply wp_let'.
     { simpl. rewrite decide_left. done. }
     iModIntro. iApply (He2 with "* HEAP LFT Htl HE HL [HC] HT"). clear He2.
     iIntros "HE". iLöb as "IH". iIntros (x) "H".
     iDestruct "H" as %[->|?]%elem_of_cons; last by iApply ("HC" with "HE *").
     iIntros (args) "Htl HL HT". iApply wp_rec; try done.
-    { apply Forall_of_val_is_val. }
-    { rewrite -vec_to_list_map -subst_vec_eq. eauto. }
+    { rewrite Forall_fmap Forall_forall=>? _. rewrite /= to_of_val. eauto. }
+    { by rewrite -vec_to_list_map -subst_v_eq. }
     (* FIXME: iNext here unfolds things in the context. *)
     iNext. iApply (Hecont with "* HEAP LFT Htl HE HL [HC] HT").
     by iApply "IH".
   Qed.
-
 End typing.
